Ackermann interface

teaching/taltech2018/code/talk/Ackermann.fst
@@ -1,8 +1,36 @@
 module Ackermann
 
-(* val ackermann: m:nat -> n:nat -> Tot nat *)
+(* This function is exposed by the interface file Ackermann.fsti, 
+   see the interface file Ackermann.fsti for its type signature.  *)
 
 let rec ackermann m n = 
   if m = 0 then n + 1
   else if n = 0 then ackermann (m - 1) 1
   else ackermann (m - 1) (ackermann m (n - 1))
+
+
+
+
+(* The following function is not exposed by the interface file Ackermann.fsti *)
+
+val swapped_ackermann: n:nat -> m:nat -> Tot nat (decreases %[m;n])
+
+let rec swapped_ackermann n m = 
+  if m = 0 then n + 1
+  else if n = 0 then swapped_ackermann 1 (m - 1)
+  else swapped_ackermann (swapped_ackermann (n - 1) m) (m - 1)
+
+
+
+
+(* The following function is not exposed by the interface file Ackermann.fsti, and 
+   as per the [@expect_failure] annotation, it is expected to fail to typecheck.   *)
+
+val swapped_ackermann_bad: n:nat -> m:nat -> Tot nat
+
+[@expect_failure] 
+let rec swapped_ackermann_bad n m = 
+  if m = 0 then n + 1
+  else if n = 0 then swapped_ackermann_bad 1 (m - 1)
+  else swapped_ackermann_bad (swapped_ackermann_bad (n - 1) m) (m - 1)
+
